InferApp.v
@@ -99,3 +99,43 @@ Lemma open_tapp:
 Proof.
   eauto using open_tapp_helper.
 Qed.
+
+Lemma open_tlet_helper:
+  forall Θ Γ t1 t2 T1 T2 x,
+    is_erased_type T2 ->
+    is_erased_term t2 ->
+    wf T1 0 ->
+    wf T2 1 ->
+    wf t2 1 ->
+    subset (fv T1) (support Γ) ->
+    subset (fv T2) (support Γ) ->
+    subset (fv t2) (support Γ) ->
+    subset (pfv_context Γ term_var) (support Γ) ->
+    ~ x ∈ support Γ ->
+    [ Θ; Γ ⊨ t1 : T1 ] ->
+    [ Θ; (x, T1) :: Γ ⊨ open 0 t2 (fvar x term_var) : open 0 T2 (fvar x term_var) ] ->
+    [ Θ; Γ ⊨ let' t1 t2 : open 0 T2 t1 ].
+Proof.
+  unfold let'; intros.
+  apply open_tapp_helper with T1 (T_arrow T1 T2); steps.
+  apply open_reducible_lambda with x; steps; eauto with wf erased fv.
+Qed.
+
+Lemma open_tlet:
+  forall Γ t1 t2 T1 T2 x,
+    is_erased_type T2 ->
+    is_erased_term t2 ->
+    wf T1 0 ->
+    wf T2 1 ->
+    wf t2 1 ->
+    subset (fv T1) (support Γ) ->
+    subset (fv T2) (support Γ) ->
+    subset (fv t2) (support Γ) ->
+    subset (pfv_context Γ term_var) (support Γ) ->
+    ~ x ∈ support Γ ->
+    [ Γ ⊨ t1 : T1 ] ->
+    [ (x, T1) :: Γ ⊨ open 0 t2 (fvar x term_var) : open 0 T2 (fvar x term_var) ] ->
+    [ Γ ⊨ let' t1 t2 : open 0 T2 t1 ].
+Proof.
+  eauto using open_tlet_helper.
+Qed.
