README.md
@@ -41,7 +41,7 @@ The typing algorithm maintains the following invariants, which are not proven in
 We prove the following properties and the soundness of the rules used in our algorithm.
 
 * Properties: 2/3
-* Rules: 27/29
+* Rules: 29/29
 
 #### Required properties (2/3)
 
@@ -64,33 +64,32 @@ We prove the following properties and the soundness of the rules used in our alg
 * NMatch3: `open_nmatch_3` in [NormalizationMatch.v](NormalizationMatch.v)
 
 
-#### Inference Rules (8/9)
+#### Inference Rules (9/9)
 
 * TVar: `open_tvar` in [InferMisc.v](InferMisc.v)
+* TAbs: `open_tabs` in [InferMisc.v](InferMisc.v)
+* TApp: `open_tapp` in [InferApp.v](InferApp.v)
+* TLet `open_tlet` in [InferApp.v](InferApp.v)
 * TNil: `open_tnil` in [ErasedList.v](ErasedList.v)
 * TCons: `open_tcons` in [ErasedList.v](ErasedList.v)
-* TCheck: `open_subtype_reducible` in [ReducibilitySubtype.v](ReducibilitySubtype.v)
-* TAbs: `open_tabs` in [InferMisc.v](InferMisc.v)
 * TFix: `open_tfix` in [InferFix.v](InferFix.v)
 * TMatch: `open_tmatch` in [InferMatch.v](InferMatch.v)
-* TApp: `open_tapp` in [InferApp.v](InferApp.v)
+* TCheck: `open_subtype_reducible` in [ReducibilitySubtype.v](ReducibilitySubtype.v)
 
-* TLet (WIP)
 
-#### Subtyping Rules (10/11)
+#### Subtyping Rules (11/11)
 
 * SubTop: `open_subtype` in [SubtypeMisc.v](SubtypeMisc.v)
 * SubRefl: `open_subrefl` in [SubtypeMisc.v](SubtypeMisc.v)
 * SubSing: `open_subsing` in [SubtypeMisc.v](SubtypeMisc.v)
 * SubCons1: `open_subcons1` in [SubtypeList.v](SubtypeList.v)
+* SubCons2: `open_subcons2` in [SubtypeList.v](SubtypeList.v)
 * SubPi: `open_subpi` in [SubtypePi.v](SubtypePi.v)
 * SubExistsLeft: `open_sub_exists_left` in [SubtypeExists](SubtypeExists.v)
 * SubExistsRight: `open_sub_exists_right` in [SubtypeExists](SubtypeExists.v)
 * SubMatch: `open_submatch` in [SubtypeMatch.v](SubtypeMatch.v)
 * SubNormWiden: `open_subnormwiden` in [SubtypeNorm.v](SubtypeNorm.v)
 * SubNorm: `open_subnorm` in [SubtypeNorm.v](SubtypeNorm.v)
-
-* SubCons2 (WIP)
 
 
 [larabot-img]: http://laraquad4.epfl.ch:9000/epfl-lara/SystemFR/status/master
